Updated files for thesis

Algebra.thy
@@ -36,112 +36,99 @@ begin
   lemma par_subdistr: "z \<parallel> x \<le> z \<parallel> (x + y)"
     by (metis par_comm par_subdistl)
 
-  lemma par_double_iso [intro]: "w \<le> x \<Longrightarrow> y \<le> z \<Longrightarrow> w \<parallel> y \<le> x \<parallel> z"
+  lemma par_double_iso [intro!]: "w \<le> x \<Longrightarrow> y \<le> z \<Longrightarrow> w \<parallel> y \<le> x \<parallel> z"
     by (metis order_trans par_isol par_isor)
 
 end
 
 class weak_trioid = par_dioid + dioid_one_zerol
 
-class trioid = par_dioid + dioid_one_zero + complete_lattice
-
-locale rg_algebra =
-  fixes restrict :: "'b::complete_lattice \<Rightarrow> 'a::trioid \<Rightarrow> 'a::trioid" (infixr "\<Colon>" 55)
-  and rg :: "'b::complete_lattice \<Rightarrow> 'a::trioid \<Rightarrow> 'a::trioid" (infixr "\<leadsto>" 55)
-  and guar :: "'b::complete_lattice \<Rightarrow> 'a::trioid"
-  assumes mod_coext: "r \<Colon> x \<le> x"
-  and guar_iso: "r \<le> s \<Longrightarrow> guar r \<le> guar s"
-  and mod_top: "top \<Colon> x = x"
-  and rg_top: "top \<leadsto> x = x"
-  and mod_inter: "r \<sqinter> s \<Colon> x = r \<Colon> s \<Colon> x"
-  and mod_isotone: "r \<le> s \<Longrightarrow> r \<Colon> x \<le> s \<Colon> x"
-  and galois: "(r \<Colon> x \<le> y) \<longleftrightarrow> (x \<le> r \<leadsto> y)"
-  and rg_antitone: "r \<le> s  \<Longrightarrow> s \<leadsto> x \<le> r \<leadsto> x"
-  and guar_par: "guar g1 \<parallel> guar g2 = guar (g1 \<squnion> g2)"
-
-  and rg_axiom: "r \<Colon> (r \<squnion> g2 \<leadsto> guar g1 \<sqinter> x) \<parallel> (r \<squnion> g1 \<leadsto> guar g2 \<sqinter> y) \<le> (guar g1 \<sqinter> x) \<parallel> (guar g2 \<sqinter> y)"
+class trioid = par_dioid + left_kleene_algebra + residual_r_op +
+  fixes meet :: "'a \<Rightarrow> 'a \<Rightarrow> 'a"  (infixl "\<otimes>" 69)
+  assumes meet_leq: "(x \<le> y) \<longleftrightarrow> (x = x \<otimes> y)"
+  and meet_assoc: "(x \<otimes> y) \<otimes> z = x \<otimes> (y \<otimes> z)"
+  and meet_sym: "x \<otimes> y = y \<otimes> x"
+  and preimp_galois: "x \<cdot> y \<le> z \<longleftrightarrow> y \<le> x \<rightarrow> z"
 
 begin
 
-  lemma rg_axiom_var: "(r \<squnion> g2 \<leadsto> guar g1 \<sqinter> x) \<parallel> (r \<squnion> g1 \<leadsto> guar g2 \<sqinter> y) \<le> r \<leadsto> (guar g1 \<sqinter> x) \<parallel> (guar g2 \<sqinter> y)"
-    by (metis galois rg_axiom)
+  lemma meet_idem [simp]: "x \<otimes> x = x"
+    by (metis local.meet_leq local.order_refl)
 
-  lemma rg_ext: "x \<le> r \<leadsto> x"
-    by (metis galois mod_coext)
+  lemma meet_1 [simp]: "x \<otimes> y \<le> y"
+    by (simp add: meet_leq meet_assoc)
 
-  lemma mod_prog_iso: "x \<le> y \<Longrightarrow> r \<Colon> x \<le> r \<Colon> y"
-    by (metis ab_semigroup_add_class.add_ac(1) dual_order.order_iff_strict galois order_prop)
+  lemma meet_2 [simp]: "y \<otimes> x \<le> y"
+    by (metis local.meet_sym meet_1)
 
-  lemma rg_prog_iso: "x \<le> y \<Longrightarrow> r \<leadsto> x \<le> r \<leadsto> y"
-    by (metis dual_order.trans galois order_refl)
+  lemma preimp_isor: "x \<le> y \<Longrightarrow> p \<rightarrow> x \<le> p \<rightarrow> y"
+    by (metis local.order.trans local.order_refl local.preimp_galois)
 
-  lemma rg_mono: "r \<le> s \<Longrightarrow> x \<le> y \<Longrightarrow> s \<leadsto> x \<le> r \<leadsto> y"
-    by (metis galois rg_antitone sup.coboundedI1 sup.orderE sup_commute)
+  lemma meet_is_meet: "x \<le> y \<otimes> z \<longleftrightarrow> (x \<le> y) \<and> (x \<le> z)"
+    by (metis (poly_guards_query) local.meet_assoc local.meet_leq local.meet_sym meet_idem)
 
-  lemma "r \<squnion> s \<leadsto> x \<le> r \<leadsto> s \<leadsto> x"
-    apply (rule rg_mono)
-    apply (metis sup.cobounded1)
-    by (metis rg_ext)
+  lemma meet_interchange: "(x \<otimes> y) \<parallel> (z \<otimes> w) \<le> (x \<parallel> z) \<otimes> (y \<parallel> w)"
+    by (auto simp add: meet_is_meet)
 
-  lemma "r \<Colon> r \<leadsto> x \<le> r \<Colon> x"
-    by (metis galois inf_idem mod_inter mod_prog_iso order_refl)
+  lemma meet_iso: "x \<le> y \<Longrightarrow> z \<le> w \<Longrightarrow> x \<otimes> z \<le> y \<otimes> w"
+    by (metis local.meet_leq meet_idem meet_is_meet)
 
-  definition quintuple :: "'b \<Rightarrow> 'b \<Rightarrow> 'a \<Rightarrow> 'a \<Rightarrow> 'a \<Rightarrow> bool" ("_, _ \<turnstile> \<lbrace>_\<rbrace> _ \<lbrace>_\<rbrace>" [20,20,20,20,20] 1000) where
-    "r, g \<turnstile> \<lbrace>p\<rbrace> x \<lbrace>q\<rbrace> \<equiv> (p \<cdot> x \<le> r \<leadsto> guar g \<sqinter> q) \<and> (guar r \<parallel> q \<le> q)"
+  lemma absorb1: "x \<otimes> (x + y) = x"
+    by (rule antisym) (simp add: meet_is_meet)+
+    
+  lemma absorb2: "x + (x \<otimes> y) = x"
+    by (metis add_commute local.less_eq_def meet_2)
 
-  lemma "r \<Colon> r \<leadsto> x \<le> r \<Colon> x"
-    by (metis galois inf_idem mod_inter mod_prog_iso order_refl)
+end 
 
-  lemma "r \<leadsto> x \<le> r \<leadsto> r \<Colon> x"
-    by (metis galois inf_idem mod_inter mod_prog_iso order_refl)
+locale rg_algebra =
+  fixes rg :: "'b::complete_lattice \<Rightarrow> 'a::trioid \<Rightarrow> 'a::trioid" (infixr "\<rhd>" 55)
+  and guar :: "'b::complete_lattice \<Rightarrow> 'a::trioid"
+  assumes rely_mult: "(r \<rhd> x) \<cdot> (r \<rhd> y) \<le> r \<rhd> (x \<cdot> y)"
+  and rely_star: "(r \<rhd> x)\<^sup>\<star> \<le> r \<rhd> (x\<^sup>\<star>)"
+  and rely_iso: "x \<le> y \<Longrightarrow> r \<rhd> x \<le> r \<rhd> y"
+  and rely_coext: "x \<le> r \<rhd> x"
+  and rely_idem: "r \<rhd> r \<rhd> x = r \<rhd> x"
+  and rely_anti: "r \<le> g \<Longrightarrow> g \<rhd> x \<le> r \<rhd> x"
+  and guar_par: "guar r \<parallel> guar g \<le> guar (r \<squnion> g)"
+  and guar_mult: "guar r \<cdot> guar g \<le> guar (r \<squnion> g)"
+  and guar_star: "(guar g)\<^sup>\<star> = guar g"
+  and guar_meet: "(x \<otimes> guar g) \<cdot> (y \<otimes> guar g) = x\<cdot>y \<otimes> guar g"
+  and rely_guarantee: "(r \<squnion> g\<^sub>2 \<rhd> x \<otimes> guar g\<^sub>1) \<parallel> (r \<squnion> g\<^sub>1 \<rhd> y \<otimes> guar g\<^sub>2) \<le> r \<rhd> (x \<otimes> guar g\<^sub>1) \<parallel> (y \<otimes> guar g\<^sub>2)"
+  and guar_iso: "r \<le> s \<Longrightarrow> guar r \<le> guar s"
 
-  lemma rely_swap: "r \<Colon> r \<leadsto> x \<le> r \<leadsto> r \<Colon> x"
-    by (metis galois order_refl rg_prog_iso)
+begin
 
-  theorem parallel_rule:
-    assumes "r \<squnion> g1 \<le> r2"
-    and "r \<squnion> g2 \<le> r1"
-    and "g1 \<squnion> g2 \<le> g"
-    and "r1, g1 \<turnstile> \<lbrace>p\<rbrace> x \<lbrace>q1\<rbrace>"
-    and "r2, g2 \<turnstile> \<lbrace>p\<rbrace> y \<lbrace>q2\<rbrace>"
-    and "p \<cdot> (x \<parallel> y) \<le> p \<cdot> x \<parallel> p \<cdot> y"
-    shows "r, g \<turnstile> \<lbrace>p\<rbrace> x \<parallel> y \<lbrace>q1 \<sqinter> q2\<rbrace>"
-  proof -
-    from assms(5) have g1_preserves_q2: "guar g1 \<parallel> q2 \<le> q2"
-      by (simp add: quintuple_def) (metis assms(1) dual_order.trans guar_iso par_isol sup.boundedE)
+definition quintuple :: "'b \<Rightarrow> 'b \<Rightarrow> 'a \<Rightarrow> 'a \<Rightarrow> 'a \<Rightarrow> bool" ("_, _ \<turnstile> \<lbrace>_\<rbrace> _ \<lbrace>_\<rbrace>" [20,20,20,20,20] 1000) where
+    "r, g \<turnstile> \<lbrace>p\<rbrace> x \<lbrace>q\<rbrace> \<equiv> (x \<le> p \<rightarrow> (r \<rhd> q \<otimes> guar g))"
 
-    from assms(5) have r2_preserves_q2: "guar r2 \<parallel> q2 \<le> q2"
-      by (simp add: quintuple_def)
-
-    from assms(4) have g2_preserves_q1: "q1 \<parallel> guar g2 \<le> q1"
-      by (simp add: quintuple_def) (metis assms(2) guar_iso par_comm par_isor sup.boundedE sup_absorb2)
-
-    from assms(4) have r1_preserves_q1: "guar r1 \<parallel> q1 \<le> q1"
-      by (simp add: quintuple_def)
-
-    have "p \<cdot> (x \<parallel> y) \<le> p \<cdot> x \<parallel> p \<cdot> y"
-      by (metis assms(6))
-    also have "... \<le> (r1 \<leadsto> guar g1 \<sqinter> q1) \<parallel> (r2 \<leadsto> guar g2 \<sqinter> q2)"
-      by (metis assms(4) assms(5) par_double_iso quintuple_def)
-    also have "... \<le> (r \<squnion> g2 \<leadsto> guar g1 \<sqinter> q1) \<parallel> (r \<squnion> g1 \<leadsto> guar g2 \<sqinter> q2)"
-      by (metis assms(1) assms(2) par_double_iso rg_antitone)
-    also have "... \<le> r \<leadsto> (guar g1 \<sqinter> q1) \<parallel> (guar g2 \<sqinter> q2)"
-      by (metis rg_axiom_var)
-    also have "... \<le> r \<leadsto> guar (g1 \<squnion> g2) \<sqinter> (q1 \<sqinter> q2)"
-      apply (auto intro!: rg_prog_iso)
-      apply (metis guar_par inf.cobounded2 inf_commute par_double_iso)
-      apply (metis g2_preserves_q1 inf_commute inf_sup_ord(2) order.trans par_double_iso)
-      by (metis g1_preserves_q2 inf.bounded_iff inf.cobounded2 inf_absorb2 par_double_iso)
-    finally have "p \<cdot> (x \<parallel> y) \<le> r \<leadsto> guar (g1 \<squnion> g2) \<sqinter> (q1 \<sqinter> q2)" .
-    moreover have "guar r \<parallel> q1 \<sqinter> q2 \<le> q1 \<sqinter> q2"
-      apply auto
-      apply (metis assms(2) guar_iso inf_sup_ord(1) order_trans par_double_iso r1_preserves_q1 sup.boundedE)
-      by (metis assms(1) guar_iso inf_sup_ord(2) order_trans par_double_iso r2_preserves_q2 sup.boundedE)
-    ultimately show ?thesis
-      apply (simp add: quintuple_def)
-      apply (erule order_trans)
-      by (metis assms(3) guar_iso inf_mono order_refl rg_prog_iso)
-  qed
+lemma parallel_rule:
+  assumes test_interchange: "\<And>x y. (p\<^sub>1 \<rightarrow> x) \<parallel> (p\<^sub>2 \<rightarrow> y) \<le> (p\<^sub>1 \<otimes> p\<^sub>2) \<rightarrow> (x \<parallel> y)"
+  and test_post: "(q\<^sub>1 \<parallel> q\<^sub>2) \<otimes> guar g \<le> r \<rhd> q\<^sub>1 \<otimes> q\<^sub>2 \<otimes> guar g"
+  and "r \<squnion> g\<^sub>1 \<le> r\<^sub>2" and "r \<squnion> g\<^sub>2 \<le> r\<^sub>1"
+  and "g\<^sub>1 \<squnion> g\<^sub>2 \<le> g"
+  and left_prog: "r\<^sub>1, g\<^sub>1 \<turnstile> \<lbrace>p\<^sub>1\<rbrace> x \<lbrace>q\<^sub>1\<rbrace>"
+  and right_prog: "r\<^sub>2, g\<^sub>2 \<turnstile> \<lbrace>p\<^sub>2\<rbrace> y \<lbrace>q\<^sub>2\<rbrace>"
+  shows "r, g \<turnstile> \<lbrace>p\<^sub>1 \<otimes> p\<^sub>2\<rbrace> x \<parallel> y \<lbrace>q\<^sub>1 \<otimes> q\<^sub>2\<rbrace>"
+proof -
+  have "x \<parallel> y \<le> (p\<^sub>1 \<rightarrow> (r\<^sub>1 \<rhd> q\<^sub>1 \<otimes> guar g\<^sub>1)) \<parallel> (p\<^sub>2 \<rightarrow> (r\<^sub>2 \<rhd> q\<^sub>2 \<otimes> guar g\<^sub>2))"
+    by (metis left_prog par_double_iso quintuple_def right_prog)
+  also have "... \<le> p\<^sub>1 \<otimes> p\<^sub>2 \<rightarrow> (r\<^sub>1 \<rhd> q\<^sub>1 \<otimes> guar g\<^sub>1) \<parallel> (r\<^sub>2 \<rhd> q\<^sub>2 \<otimes> guar g\<^sub>2)"
+    by (rule test_interchange)
+  also have "... \<le> p\<^sub>1 \<otimes> p\<^sub>2 \<rightarrow> (r \<squnion> g\<^sub>2 \<rhd> q\<^sub>1 \<otimes> guar g\<^sub>1) \<parallel> (r \<squnion> g\<^sub>1 \<rhd> q\<^sub>2 \<otimes> guar g\<^sub>2)"
+    by (metis assms(3) assms(4) par_double_iso preimp_isor rely_anti)
+  also have "... \<le> p\<^sub>1 \<otimes> p\<^sub>2 \<rightarrow> (r \<rhd> (q\<^sub>1 \<otimes> guar g\<^sub>1) \<parallel> (q\<^sub>2 \<otimes> guar g\<^sub>2))"
+    by (metis preimp_isor rely_guarantee)
+  also have "... \<le> p\<^sub>1 \<otimes> p\<^sub>2 \<rightarrow> (r \<rhd> (q\<^sub>1 \<parallel> q\<^sub>2) \<otimes> (guar g\<^sub>1 \<parallel> guar g\<^sub>2))"
+    by (intro preimp_isor rely_iso meet_interchange)
+  also have "... \<le> p\<^sub>1 \<otimes> p\<^sub>2 \<rightarrow> (r \<rhd> (q\<^sub>1 \<parallel> q\<^sub>2) \<otimes> guar g)"
+    by (metis (poly_guards_query) assms(5) guar_iso guar_par meet_2 meet_is_meet meet_sym order_trans preimp_isor rely_iso)
+  also have "... \<le> p\<^sub>1 \<otimes> p\<^sub>2 \<rightarrow> (r \<rhd> (q\<^sub>1 \<otimes> q\<^sub>2) \<otimes> guar g)"
+    by (metis preimp_isor rely_idem rely_iso test_post)
+  finally have "x \<parallel> y \<le> p\<^sub>1 \<otimes> p\<^sub>2 \<rightarrow> (r \<rhd> (q\<^sub>1 \<otimes> q\<^sub>2) \<otimes> guar g)" .
+  thus ?thesis
+    by (simp only: quintuple_def[symmetric])
+qed
 
 end
 
